### Proof 1
A(1, y) = y + 2
Basis
A(1, 0) = 0 + 2 = 2
by algorithm = A(1,0) = A(1,0) = 1 + 1 = 2
Therefore basis is true
### Hypothesis
Assume for all y = k, k is an element of N, A(1,k) = k+2 is true

### Inductive Step
for y = k + 1
A(1, k + 1) = A(0, A(1, k))
= A(0, k + 2) -> (A(0,y) = y + 1)
= k + 2 + 1 = k +3
= (k + 1) + 2

### Conclusion
From the basis and the inductive steps,
it follows that the inductive hypothesis hold for every value
y = k, for all elements of k in N


### Proof 2
Basis
for y = 0
A(2,0) = 3
According to algorithm
A(2,0) = A(1,1) according to proof A(1, 1) = 1 + 2 = 3
Basis is true

### Inductive Hypothesis
Assume for y = k, y is an element of N, the statement

### Inductive Step
for y = k + 1
A(2, k + 1) = A(1, A(2,k)) = A(1, 2k + 3)
Using Proof (1):
A(1, 2k+3) = 2k + 3 + 2 = 2(k+1) +3

### Conclusion
The inductive hypothesis holds true for all y elements of N


### Proof 3
A(3, y) = 2^(y + 3) - 3

Basis
for y = 0
A(3,0) = 2^3 - 3 = 5
According to the algorithm
A(3, 0) = A(2,0) using proof (2)
A(2, 1) = 2(1) + 3 = 5
Basis is true

### Hypothesis
Assume for y = k, where k is an element of N, the statement
A(3, k) = 2^(k+3) - 3

### Inductive Steps
for y = k + 1
A(3, k+1) = A(2, A(3, k))
= A(2, 2^(k+3) - 3)
Using proof (2)
A(2, 2^(k+3) - 3) = 2(2^(k+3) + 3)
= 2^(k+3).2^1-6+3
=2^(k+1) - 3
= 2^((k+1)+3) - 3

### Conclusion
The inductive hypothesis holds true for all y elements of N
